open import Function using (_âˆ˜_; id)
open import Relation.Binary.PropositionalEquality

open import Data.Nat as Nat using (â„•; zero; _+_) renaming (suc to 1+)
import Data.Nat.Properties as NatProperties
open import Data.Fin as Fin using (Fin) renaming (zero to #0; suc to #1+)


module Language.Lambda.Grammar.Definitions where


-- ================================================================
-- Definitions
-- ================================================================


infixr 15 _`â†’_

infixr 15 `_
infixr 14 `â†‘_ `â†‘+_
infixr 13 _`âˆ™_
infixr 12 `Î»_`â¦‚_`â‡’_


-- ----------------------------------------------------------------
-- Type
-- ----------------------------------------------------------------


data Type : Set where
  `ğŸ˜   : Type
  `ğŸ™   : Type
  _`â†’_ : âˆ€ (Î± Î² : Type) â†’ Type


-- examples

`ğŸ™â†’ğŸ™ : Type
`ğŸ™â†’ğŸ™ = `ğŸ™ `â†’ `ğŸ™


-- ================================================================
-- Term
-- ================================================================

-- ``t : Term n`` is a term with ``n`` free names
data Term : â„• â†’ Set where
  `1 : Term 0
  `_ : âˆ€ n  â†’ Term (1+ n)
  _`âˆ™_ : âˆ€ {n} (a b : Term n) â†’ Term n
  `Î»_`â¦‚_`â‡’_ : âˆ€ n (Î± : Type) (b : Term (1+ n)) â†’ Term n
  `â†‘_ : âˆ€ {n} (a : Term n) â†’ Term (1+ n)


-- utilities


-- if m â‰¡ n, then an m-Term is also an n-Term
cast : âˆ€ {m} {n} â†’ m â‰¡ n â†’ Term m â†’ Term n
cast mâ‰¡n t rewrite mâ‰¡n = t

`â†‘+_ : âˆ€ {m} {n} â†’ Term n â†’ Term (m + n)
`â†‘+_ {zero} {n} t = t
`â†‘+_ {1+ m} {n} t = `â†‘ (`â†‘+ t)


-- examples

`id : Term 0
`id = `Î» 0 `â¦‚ `ğŸ™ `â‡’ ` 0 -- `Î» 0 `â¦‚ `ğŸ™ `â‡’ ` 0

`const : Term 0
`const = `Î» 0 `â¦‚ `ğŸ™ `â‡’ `Î» 1 `â¦‚ `ğŸ™ `â‡’ ` 1

`apply : Term 0
`apply = `Î» 0 `â¦‚ `ğŸ™â†’ğŸ™ `â‡’ `Î» 1 `â¦‚ `ğŸ™ `â‡’ (`â†‘ ` 0) `âˆ™ ` 1

